

# AI1103-Challenging problem

Name : Aayush Patel, Roll No.: CS20BTECH11001

## QUESTION

Prove by properties of Q-function the following inequality,

$$1 - \exp(-2\pi) \geq \left(1 - 2Q\left(\frac{1}{2}\right)\right)^2$$

## SOLUTION

### Some Properties of Q function:

**Lemma 0.1.**  $Q(x) + Q(-x) = 1$

**Lemma 0.2.** Chernoff Lower Bound Property

$$Q(x) \geq f(x)$$

where  $f(x) = \alpha \exp(-\beta x^2)$  and

$$\beta > 1, 0 < \alpha \leq \frac{\sqrt{2e} \sqrt{\beta - 1}}{\sqrt{\pi}\beta}$$

Simplifying the inequality given in question,

$$1 - \exp(-2\pi) \geq \left(1 - 2Q\left(\frac{1}{2}\right)\right)^2 \quad (0.0.1)$$

$$1 - \exp(-2\pi) \geq 1 + 4Q^2\left(\frac{1}{2}\right) - 4Q\left(\frac{1}{2}\right) \quad (0.0.2)$$

$$-\exp(-2\pi) \geq 4Q\left(\frac{1}{2}\right)\left(Q\left(\frac{1}{2}\right) - 1\right) \quad (0.0.3)$$

$$\exp(-2\pi) \leq 4Q\left(\frac{1}{2}\right)\left(1 - Q\left(\frac{1}{2}\right)\right) \quad (0.0.4)$$

$$4Q\left(\frac{1}{2}\right)\left(1 - Q\left(\frac{1}{2}\right)\right) \geq \exp(-2\pi) \quad (0.0.5)$$

Using Lemma 0.1 of Q-functions,

$$Q(x) + Q(-x) = 1 \quad (0.0.6)$$

$$4Q\left(\frac{1}{2}\right)Q\left(-\frac{1}{2}\right) \geq \exp(-2\pi) \quad (0.0.7)$$

**Lemma 0.3.**  $4Q\left(\frac{1}{2}\right)Q\left(-\frac{1}{2}\right) \geq \exp(-2\pi)$

*Proof.* Using Lemma 0.2 of Q-functions and the fact that  $f(x)$  is even.

$$4Q(x\sqrt{2}) \cdot Q(-x\sqrt{2}) \geq \alpha^2 \exp(-2\beta x^2) \quad (0.0.8)$$

Putting  $x = \frac{1}{2\sqrt{2}}$ , we get,

$$4Q\left(\frac{1}{2}\right) \cdot Q\left(-\frac{1}{2}\right) \geq \alpha^2 \exp\left(\frac{-\beta}{4}\right) \quad (0.0.9)$$

For  $\beta = 8\pi$ ,

$$0 < \alpha \leq \frac{\sqrt{2e} \sqrt{8\pi - 1}}{\sqrt{\pi}8\pi} \quad (0.0.10)$$

$$(0.0.11)$$

Clearly, denominator is greater than numerator, therefore,  $\alpha < 1$

$$4Q\left(\frac{1}{2}\right) \cdot Q\left(-\frac{1}{2}\right) \geq \alpha^2 \exp(-2\pi) \quad (0.0.12)$$

where  $\alpha < 1$

Therefore,

$$4Q\left(\frac{1}{2}\right) \cdot Q\left(-\frac{1}{2}\right) \geq \exp(-2\pi) \quad (0.0.13)$$

□

Hence proved